ReactorModel/Execution/Theorems/Variability/Basic.lean
@@ -1,9 +1,6 @@
-import ReactorModel.Execution.Theorems.Step.Basic
-import ReactorModel.Execution.Theorems.State
-import ReactorModel.Execution.Theorems.Variability.LoopModel
-import ReactorModel.Execution.Theorems.Execution
+import ReactorModel.Execution.Theorems.Variability.Loop.Execution
 
-open Classical Reactor
+open Reactor
 
 namespace Execution
 
@@ -25,116 +22,14 @@ def FiniteVariability (α) [Hierarchical α] : Prop :=
   ∀ g s, ∃ b, ∀ {s' : State α} (e : Execution s s'),
     (s'.tag ≤ g) → e.length ≤ b
 
-noncomputable def LoopModel.state₀ (microstep : Nat) : State LoopModel.Rtr where
-  rtr := { act := true }
-  tag := ⟨0, microstep⟩
-  progress := ∅
-  events
-    | .r => none
-    | .a => actionEvents microstep
-where
-  actionEvents : Nat → Time.Tag ⇉ Bool
-    | 0     => .singleton ⟨0, 0⟩ true
-    | m + 1 => (actionEvents m).insert ⟨0, m + 1⟩ true
-
-open _root_.LoopModel in
-theorem LoopModel.state₀_schedule_actionEvents (m) :
-    State.schedule.go (α := Rtr) (state₀.actionEvents m) 0 true = state₀.actionEvents (m + 1) := by
-  sorry
-
--- TODO: Define a ++ operator for executions
-
-open _root_.LoopModel in
-private noncomputable def LoopModel.execution₀ :
-    (microstep : Nat) → Execution (state₀ 0) (state₀ microstep)
-  | 0     => .refl
-  | m + 1 =>
-    let e := execution₀ m
-    let s₁ := state₀ m |>.schedule .a 0 true |>.record .r
-    let s₂ := state₀ (m + 1)
-    let timeStep : s₁ ↓ₜ s₂ := sorry
-    execution₀ m |>.push (.exec <| execStep m) |>.push (.time timeStep)
-where
-  execStep (m) : (state₀ m) ↓ₑ (state₀ m |>.schedule .a 0 true |>.record .r) :=
-    .mk execStep_allows execStep_triggers execStep_apply
-  execStep_allows {m} : (state₀ m).Allows .r := {
-      mem           := by simp [Partial.mem_iff, Rtr.obj?_rcn_r]
-      deps          := by simp [dependencies, Rtr.no_deps]
-      unprocessed _ := by contradiction
-    }
-  execStep_triggers {m} : (state₀ m).Triggers .r :=
-    .intro (Rtr.obj?_rcn_r _) <| by
-      exists ⟨.act, .a⟩, true
-      simp [LoopModel.Rtr.obj?_rcn_r, Rtr.obj?_act_a, Rtr.rcn, state₀, State.input,
-            State.input.restriction, Partial.restrict]
-  execStep_apply {m} : (state₀ m) -[(state₀ m).output .r]→ (state₀ m |>.schedule .a 0 true) := by
-    simp only [Rtr.obj?_rcn_r, Rtr.rcn, State.input, State.output, Option.elim_some]
-    exact Step.Apply.RTC.trans .act .refl
-  timeStep (m) : (state₀ m |>.schedule .a 0 true |>.record .r) ↓ₜ (state₀ <| m + 1) :=
-    let s₁ := state₀ m |>.schedule .a 0 true |>.record .r
-    let s₂ := { s₁ with rtr := s₁.rtr, tag := ⟨0, m + 1⟩, progress := ∅ }
-    have h : s₂ = (state₀ <| m + 1) := by
-      simp only [state₀, State.record_preserves_rtr, State.schedule_preserves_rtr,
-                 State.record_preserves_events, State.mk.injEq, true_and, s₂, s₁, State.schedule]
-      funext i
-      cases i <;> simp only [Partial.update, reduceCtorEq, ↓reduceIte, Option.map_eq_map,
-                             Option.map_some', state₀_schedule_actionEvents, s₂, s₁]
-    h ▸ .mk timeStep_closed timeStep_next timeStep_refresh
-  timeStep_closed {m} : (state₀ m |>.schedule .a 0 true |>.record .r).Closed := by
-    rw [State.Closed, Rtr.rcn_ids]
-    simp [State.schedule_preserves_progress, State.record_progress_eq, state₀, Set.insert]
-  timeStep_next {m} : (state₀ m |>.schedule .a 0 true |>.record .r).NextTag ⟨0, m + 1⟩ := {
-      mem   := timeStep_next_mem
-      bound := sorry
-      least := sorry
-    }
-  timeStep_next_mem {m} : ⟨0, m + 1⟩ ∈ (((state₀ m).schedule .a 0 true).record .r).scheduledTags := by
-    exists .a
-    simp [State.scheduledTags, State.schedule, state₀, Partial.update, State.schedule.go, state₀.actionEvents]
-    induction m
-    case zero =>
-      simp [state₀.actionEvents]
-      split
-      · contradiction
-      next h =>
-        have ⟨h, _⟩ := Finset.mem_filter.mp <| Finset.mem_of_max h
-        simp only [Finset.mem_singleton, Time.Tag.mk.injEq] at h
-        simp [h.right, Finmap.mem_keys]
-    case succ ih =>
-      simp [state₀.actionEvents]
-      split
-      next m _ h =>
-        have := Finset.filter_eq_empty_iff.mp (Finset.max_eq_bot.mp h) (x := ⟨0, m + 1⟩) (by simp [Finmap.mem_keys])
-        contradiction
-      · sorry
-  timeStep_refresh {m} :
-      Refresh (state₀ m |>.schedule .a 0 true |>.record .r).rtr
-              (state₀ m |>.schedule .a 0 true |>.record .r).rtr
-              ((state₀ m |>.schedule .a 0 true |>.record .r).actions ⟨0, m + 1⟩) := {
-      equiv    := .refl _
-      eq_state := rfl
-      inputs   := by simp
-      outputs  := by simp
-      acts     := by
-        simp [State.actions]
-        sorry
-    }
-
-private theorem LoopModel.execution₀_length_le (microstep : Nat) :
-    microstep ≤ (execution₀ microstep).length := by
-  induction microstep
-  case zero => rfl
-  case succ => simp [execution₀, Nat.le_add_right_of_le, *]
-
 -- Properness of a finite reactor model is not sufficient for finite variability. This is a
 -- consequence of logical tags being super-dense.
 --
--- Proof Idea: Construct a reactor with a reaction which always schedules and action for the
---             current logical time. This only ever increases the micro-step, but not the time.
-open LoopModel in
+-- Proof Idea: Construct a reactor with a reaction which always schedules an action for the current
+--             logical time. This only ever increases the microstep, but not the time.
 theorem not_finitely_variable : ¬∀ (α) [Proper α] [Reactor.Finite α], FiniteVariability α := by
   intro h
-  have ⟨b, h⟩ := h _ ⟨1, 0⟩ (state₀ 0)
-  have := h (execution₀ <| b + 1) (le_of_lt <| Time.Tag.lt_of_lt_time Nat.zero_lt_one)
-  have := execution₀_length_le (b + 1)
+  have ⟨b, h⟩ := h _ ⟨1, 0⟩ (Loop.state₀ 0)
+  have := h (Loop.execution₀ <| b + 1) (le_of_lt <| Time.Tag.lt_of_lt_time Nat.zero_lt_one)
+  have := Loop.execution₀_length_le (b + 1)
   omega
