ReactorModel/Execution/Theorems/Variability/Loop/Execution.lean
@@ -1,0 +1,103 @@
+import ReactorModel.Execution.Theorems.Step.Basic
+import ReactorModel.Execution.Theorems.State
+import ReactorModel.Execution.Theorems.Variability.Loop.Reactor
+import ReactorModel.Execution.Theorems.Execution
+
+noncomputable section
+open Reactor Execution
+
+namespace Loop
+
+def state₀ (microstep : Nat) : State Reactor where
+  rtr := { act := true }
+  tag := ⟨0, microstep⟩
+  progress := ∅
+  events
+    | .r => none
+    | .a => actionEvents microstep
+where
+  actionEvents : Nat → Time.Tag ⇉ Bool
+    | 0     => .singleton ⟨0, 0⟩ true
+    | m + 1 => (actionEvents m).insert ⟨0, m + 1⟩ true
+
+theorem state₀_schedule_actionEvents (m) :
+    State.schedule.go (α := Reactor) (state₀.actionEvents m) 0 true = state₀.actionEvents (m + 1) := by
+  sorry
+
+def execution₀ : (microstep : Nat) → Execution (state₀ 0) (state₀ microstep)
+  | 0     => .refl
+  | m + 1 =>
+    let e := execution₀ m
+    let s₁ := state₀ m |>.schedule .a 0 true |>.record .r
+    let s₂ := state₀ (m + 1)
+    let timeStep : s₁ ↓ₜ s₂ := sorry
+    execution₀ m |>.push (.exec <| execStep m) |>.push (.time timeStep)
+where
+  execStep (m) : (state₀ m) ↓ₑ (state₀ m |>.schedule .a 0 true |>.record .r) :=
+    .mk execStep_allows execStep_triggers execStep_apply
+  execStep_allows {m} : (state₀ m).Allows .r := {
+      mem           := by simp [Partial.mem_iff]
+      deps          := by simp [dependencies, no_deps]
+      unprocessed _ := by contradiction
+    }
+  execStep_triggers {m} : (state₀ m).Triggers .r :=
+    .intro (obj?_rcn_r _) <| by
+      exists ⟨.act, .a⟩, true
+      simp [rcn, state₀, State.input, State.input.restriction, Partial.restrict]
+  execStep_apply {m} : (state₀ m) -[(state₀ m).output .r]→ (state₀ m |>.schedule .a 0 true) := by
+    simp only [obj?_rcn_r, rcn, State.input, State.output, Option.elim_some]
+    exact Step.Apply.RTC.trans .act .refl
+  timeStep (m) : (state₀ m |>.schedule .a 0 true |>.record .r) ↓ₜ (state₀ <| m + 1) :=
+    let s₁ := state₀ m |>.schedule .a 0 true |>.record .r
+    let s₂ := { s₁ with rtr := s₁.rtr, tag := ⟨0, m + 1⟩, progress := ∅ }
+    have h : s₂ = (state₀ <| m + 1) := by
+      simp only [state₀, State.record_preserves_rtr, State.schedule_preserves_rtr,
+                 State.record_preserves_events, State.mk.injEq, true_and, s₂, s₁, State.schedule]
+      funext i
+      cases i <;> simp only [Partial.update, reduceCtorEq, ↓reduceIte, Option.map_eq_map,
+                             Option.map_some', state₀_schedule_actionEvents, s₂, s₁]
+    h ▸ .mk timeStep_closed timeStep_next timeStep_refresh
+  timeStep_closed {m} : (state₀ m |>.schedule .a 0 true |>.record .r).Closed := by
+    rw [State.Closed, rcn_ids]
+    simp [State.schedule_preserves_progress, State.record_progress_eq, state₀, Set.insert]
+  timeStep_next {m} : (state₀ m |>.schedule .a 0 true |>.record .r).NextTag ⟨0, m + 1⟩ := {
+      mem   := timeStep_next_mem
+      bound := sorry
+      least := sorry
+    }
+  timeStep_next_mem {m} : ⟨0, m + 1⟩ ∈ (((state₀ m).schedule .a 0 true).record .r).scheduledTags := by
+    exists .a
+    simp [State.scheduledTags, State.schedule, state₀, Partial.update, State.schedule.go, state₀.actionEvents]
+    induction m
+    case zero =>
+      simp [state₀.actionEvents]
+      split
+      · contradiction
+      next h =>
+        have ⟨h, _⟩ := Finset.mem_filter.mp <| Finset.mem_of_max h
+        simp only [Finset.mem_singleton, Time.Tag.mk.injEq] at h
+        simp [h.right, Finmap.mem_keys]
+    case succ ih =>
+      simp [state₀.actionEvents]
+      split
+      next m _ h =>
+        have := Finset.filter_eq_empty_iff.mp (Finset.max_eq_bot.mp h) (x := ⟨0, m + 1⟩) (by simp [Finmap.mem_keys])
+        contradiction
+      · sorry
+  timeStep_refresh {m} :
+      Refresh (state₀ m |>.schedule .a 0 true |>.record .r).rtr
+              (state₀ m |>.schedule .a 0 true |>.record .r).rtr
+              ((state₀ m |>.schedule .a 0 true |>.record .r).actions ⟨0, m + 1⟩) := {
+      equiv    := .refl _
+      eq_state := rfl
+      inputs   := by simp
+      outputs  := by simp
+      acts     := by
+        simp [State.actions]
+        sorry
+    }
+
+theorem execution₀_length_le (microstep : Nat) : microstep ≤ (execution₀ microstep).length := by
+  induction microstep
+  case zero => rfl
+  case succ => simp [execution₀, Nat.le_add_right_of_le, *]
